Splinter/Journal/AllocationJournalRefinement.i.dfy
@@ -1,0 +1,204 @@
+// Copyright 2018-2021 VMware, Inc., Microsoft Inc., Carnegie Mellon University, ETH Zurich, and University of Washington
+// SPDX-License-Identifier: BSD-2-Clause
+
+include "AllocationJournal.i.dfy"
+include "LikesJournalRefinement.i.dfy"
+
+// A Journal that keeps an in-memory index that maps each in-use LSN to the Address that stores it.
+// The impl will keep such an index so that Discard can return freed Addresses without having to
+// fault in the freed section of the journal to learn the chain of addresses involved.
+module AllocationJournalRefinment {
+  import opened Options
+  import opened LSNMod
+  import opened AllocationJournal
+  import opened MiniAllocatorMod
+  import L = LikesJournal
+  import LR = LikesJournalRefinement
+
+  function I(v: Variables) : L.Variables
+  {
+    v.journal
+  }
+
+  function GetTj(v: Variables) : TruncatedJournal
+  {
+    v.journal.journal.truncatedJournal
+  }
+
+  predicate AddrIndexConsistentWithAUIndex(lsnAddrIndex: map<LSN, Address>, lsnAUIndex: map<LSN, AU>)
+  {
+    && lsnAddrIndex.Keys == lsnAUIndex.Keys
+    // Note: we need this instead of au in lsnAUIndex otherwise we can't prove DiscardOld refines
+    && (forall lsn | lsn in lsnAddrIndex :: lsnAddrIndex[lsn].au == lsnAUIndex[lsn])
+  }
+
+  predicate JournalPagesNotFree(addrs: set<Address>, allocator: MiniAllocator)
+  {
+    && (forall addr | addr in addrs :: !allocator.CanAllocate(addr))
+  }
+
+  // TODO(Jialin): bad name?
+  predicate MiniAllocatorFollowfreshestRec(freshestRec: Pointer, allocator: MiniAllocator)
+  {
+    // if freshestRec.None? then allocator.curr.None?
+    // else if freshestRec.Some? && allocator.curr.Some? 
+    // then allocator.MinAddr(freshestRec.value.NextPage())
+    // else true
+    && (freshestRec.None? ==> allocator.curr.None?)
+    && (freshestRec.Some? && allocator.curr.Some? ==> 
+      && var nextAddr := freshestRec.value.NextPage();
+      && allocator.MinAddr(nextAddr))
+  }
+
+  predicate InternalAUPagesFullyLinked(dv: DiskView, first: AU)
+  {
+    && (forall addr | addr in dv.entries && addr.au != first :: AUPagesLinkedTillFirstInOrder(dv, addr))
+    // forall addr | addr in addrs && addr.au != first :: AUPagesLinkedInOrder(dv, addr)
+  }
+
+  predicate Inv(v: Variables)
+  {
+    && LR.Inv(v.journal)
+    // relationship between lsnAddrIndex and lsnAUIndex
+    && AddrIndexConsistentWithAUIndex(v.journal.lsnAddrIndex, v.lsnAUIndex)
+    // relationship between lsnAddrIndex and miniAllocator status
+    && JournalPagesNotFree(v.journal.lsnAddrIndex.Values, v.miniAllocator)
+    // relationship between journal freshestRec and miniAllocator
+    && MiniAllocatorFollowfreshestRec(GetTj(v).freshestRec, v.miniAllocator)
+    // constraints on page links within an AU
+    // when one follows the prior link of a page within any AU except first
+    // it will observe a link that's strictly decreasing and links down to page 0
+    && InternalAUPagesFullyLinked(GetTj(v).diskView, v.first)
+
+    // To be deleted
+    // && (forall addr | addr in v.journal.lsnAddrIndex.Values :: 
+    //   && addr.au in v.lsnAUIndex.Values
+    //   && !v.miniAllocator.CanAllocate(addr))
+    // NOTE: may need to change to diskview for easier proof?
+    // && (forall addr | addr in v.journal.lsnAddrIndex.Values && addr.au != v.first ::
+    //   && AUPagesLinkedInOrder(v.journal.journal.truncatedJournal.diskView, addr))
+  }
+
+  lemma InternalJournalMarshalRefines(v: Variables, v': Variables, lbl: TransitionLabel, step: Step)
+    requires Inv(v)
+    requires InternalJournalMarshal(v, v', lbl, step)
+    ensures L.InternalJournalMarshal(I(v), I(v'), lbl.I(), step.cut, step.addr)
+    ensures Inv(v')
+  {
+    assert LR.Inv(v.journal);
+    LR.InvNextMarshalStep(I(v), I(v'), lbl.I(), step.cut, step.addr);
+    assert LR.Inv(v'.journal);
+
+    assert v.miniAllocator.MinAddr(step.addr); // 
+    
+    assert LR.IndexDomainValid(v'.journal.lsnAddrIndex, GetTj(v')); // from LR.Inv
+    var discardmsgs := v.journal.journal.unmarshalledTail.DiscardRecent(step.cut);
+    assert LikesJournal.LsnDisjoint(v.lsnAUIndex.Keys, discardmsgs) by {
+      LR.reveal_IndexDomainValid();
+    }
+    assert v'.lsnAUIndex.Values == v.lsnAUIndex.Values + {step.addr.au};
+    assert v'.journal.lsnAddrIndex.Values == v.journal.lsnAddrIndex.Values + {step.addr};
+    assert AddrIndexConsistentWithAUIndex(v'.journal.lsnAddrIndex, v'.lsnAUIndex);
+
+    // verifies just takes a while
+    assume JournalPagesNotFree(v'.journal.lsnAddrIndex.Values, v'.miniAllocator);
+
+    // assert MiniAllocatorFollowfreshestRec(GetTj(v).freshestRec, v.miniAllocator);
+    // assert GetTj(v).freshestRec.None? ==> v.miniAllocator.curr.None?;
+    // takes way too long to verify
+
+    assume MiniAllocatorFollowfreshestRec(GetTj(v').freshestRec, v'.miniAllocator);
+    // assert InternalAUPagesFullyLinked(GetTj(v').diskView, v'.first);
+
+    assert GetTj(v').diskView == GetTj(v).diskView.(entries :=
+      GetTj(v).diskView.entries[step.addr := 
+      LinkedJournal.JournalRecord(discardmsgs, GetTj(v).freshestRec)]);
+
+    forall addr | addr in GetTj(v').diskView.entries && addr.au != v'.first 
+      ensures AUPagesLinkedTillFirstInOrder(GetTj(v').diskView, addr)
+    {
+      if addr in GetTj(v).diskView.entries {
+        assert AUPagesLinkedTillFirstInOrder(GetTj(v).diskView, addr);
+      } else {
+        assert addr == step.addr;
+        if GetTj(v).freshestRec.None? {
+          // Jialin: all these assumes are asserts but idk why they take so long to verify
+          assume v.miniAllocator.curr.None?; 
+          assume v.miniAllocator.allocs[addr.au].MinFreeAddr(addr);
+          assume v.miniAllocator.allocs[addr.au]
+          v.miniAllocator.allocs[addr.au].MinFreeAddrZeroLemma(addr); 
+          assert addr.page == 0;
+          assume false;
+        } else {
+          assume false;
+        }
+
+//  && var newAddr := GenericDisk.Address(addr.au, page);
+//       && var priorAddr := GenericDisk.Address(addr.au, page-1);
+//       && dv.Decodable(Some(newAddr))
+//       && dv.entries[newAddr].CroppedPrior(dv.boundaryLSN) == Some(priorAddr))
+//   }
+
+        // we know cropped prior is fine 
+
+        // assume false;
+      }
+    }
+
+
+
+
+    // // relationship between journal freshestRec and miniAllocator
+    // && MiniAllocatorFollowfreshestRec(GetTj(v).freshestRec, v.miniAllocator)
+    // // constraints on page links within an AU
+    // // when one follows the prior link of a page within any AU except first
+    // // it will observe a link that's strictly decreasing and links down to page 0
+    // && InternalAUPagesFullyLinked(GetTj(v).diskView, v.first)
+
+  
+    // assume false;
+
+    // forall addr | addr in v'.journal.lsnAddrIndex.Values && addr.au != v'.first
+    //   ensures AUPagesLinkedInOrder(v'.journal.journal.truncatedJournal.diskView, addr)
+    // {
+    //   if addr in v.journal.lsnAddrIndex.Values {
+    //     assert AUPagesLinkedInOrder(v'.journal.journal.truncatedJournal.diskView, addr);
+    //   } else {
+
+    //     assert addr == v'.journal.journal.truncatedJournal.freshestRec.value;
+    //     assert v'.journal.journal.truncatedJournal.diskView.entries[addr].CroppedPrior(v'.journal.journal.truncatedJournal.diskView.boundaryLSN) == v.journal.journal.truncatedJournal.freshestRec;
+
+    //     var fr := v.journal.journal.truncatedJournal.freshestRec;
+    //     if fr.None? {
+    //       // we need to prove that page # is 0
+
+    //       // cur.Some? 
+    //       // connect freshest rec 
+    //     }
+
+    //     // if no record, mini allocator can't have a curr
+    //     // 
+
+    //     // invariants on the state of mini allocator?
+
+
+    //     // assert fr.Some?;
+    //     // assume addr == GenericDisk.Address(fr.value.au, fr.value.page+1);
+    //     // assume v.journal.journal.truncatedJournal.freshestRec == Some(GenericDisk.Address(addr.au, addr.page-1));
+
+    //     assume false;
+    //   }
+    // }
+
+    assume false;
+  }
+
+  lemma InitRefines()
+  {
+
+  }
+
+
+
+
+}
